remove assume in poly1305_encode

code/experimental/poly1305/Hacl.Impl.Poly1305.Lemmas.fst
@@ -75,3 +75,81 @@ let uints_to_bytes_le_lemma64_1 lo hi = admit()
 let uints_to_bytes_le_lemma64_2 r = admit()
 
 let uints_to_bytes_le_lemma128_2 r = admit()
+
+val lemma_nat_from_bytes_le_zeroes: len:size_nat -> b:lseq uint8 len -> Lemma
+  (requires (forall (i:nat). i < len ==> b.[i] == u8 0))
+  (ensures  nat_from_intseq_le_ b == 0)
+let rec lemma_nat_from_bytes_le_zeroes len b =
+  if len = 0 then ()
+  else lemma_nat_from_bytes_le_zeroes (len-1) (Seq.slice b 1 len)
+
+#set-options "--z3rlimit 50"
+
+val lemma_nat_from_bytes_le_slice0: len:size_nat{len > 0} -> b:lseq uint8 len -> i:nat{0 < i /\ i < len} -> Lemma
+  (pow2 ((i - 1) * 8) * nat_from_intseq_le_ (Seq.slice b (i - 1) len) ==
+   pow2 ((i - 1) * 8) * v b.[i - 1] + pow2 (i * 8) * nat_from_intseq_le_ (Seq.slice b i len))
+let lemma_nat_from_bytes_le_slice0 len b i =
+  assert (nat_from_intseq_le_ (Seq.slice b (i - 1) len) == v b.[i - 1] + pow2 8 * nat_from_intseq_le_ (Seq.slice b i len));
+  assert (pow2 ((i - 1) * 8) * nat_from_intseq_le_ (Seq.slice b (i - 1) len) == pow2 ((i - 1) * 8) * (v b.[i - 1] + pow2 8 * nat_from_intseq_le_ (Seq.slice b i len)));
+  FStar.Math.Lemmas.distributivity_add_right (pow2 ((i - 1) * 8)) (v b.[i - 1]) (pow2 8 * nat_from_intseq_le_ (Seq.slice b i len));
+  FStar.Math.Lemmas.paren_mul_right (pow2 ((i - 1) * 8)) (pow2 8) (nat_from_intseq_le_ (Seq.slice b i len));
+  assert (pow2 ((i - 1) * 8) * (v b.[i - 1] + pow2 8 * nat_from_intseq_le_ (Seq.slice b i len)) ==
+    pow2 ((i - 1) * 8) * v b.[i - 1] + pow2 ((i - 1) * 8) * pow2 8 * nat_from_intseq_le_ (Seq.slice b i len));
+  FStar.Math.Lemmas.pow2_plus ((i - 1) * 8) 8;
+  assert ((i-1) * 8 + 8 = i * 8);
+  assert (pow2 ((i - 1) * 8) * pow2 8 == pow2 (i * 8));
+  assert (pow2 ((i - 1) * 8) * (v b.[i - 1] + pow2 8 * nat_from_intseq_le_ (Seq.slice b i len)) ==
+    pow2 ((i - 1) * 8) * v b.[i - 1] + pow2 (i * 8) * nat_from_intseq_le_ (Seq.slice b i len))
+
+val lemma_nat_from_bytes_le_slice1: len:size_nat -> b:lseq uint8 len -> i:size_nat{0 < i /\ i < len} ->
+  Lemma
+    (requires (let b1 = Seq.slice b 0 i in
+      nat_from_intseq_le_ b1 == nat_from_intseq_le_ (Seq.slice b1 0 (i - 1)) + pow2 ((i - 1) * 8) * nat_from_intseq_le_ (Seq.slice b1 (i - 1) i)))
+    (ensures nat_from_intseq_le_ (Seq.slice b 0 i) == nat_from_intseq_le_ (Seq.slice b 0 (i - 1)) + pow2 ((i - 1) * 8) * v b.[i - 1])
+let lemma_nat_from_bytes_le_slice1 len b i = ()
+
+
+val lemma_nat_from_bytes_le_slice: len:size_nat -> b:lseq uint8 len -> i:nat{i < len} ->
+  Lemma (ensures (nat_from_intseq_le_ b == nat_from_intseq_le_ (Seq.slice b 0 i) + pow2 (i * 8) * nat_from_intseq_le_ (Seq.slice b i len)))
+let rec lemma_nat_from_bytes_le_slice len b i =
+  if len = 0 then ()
+  else begin
+    if i = 0 then begin
+      assert (nat_from_intseq_le_ (Seq.slice b 0 0) = 0);
+      assert_norm (pow2 (i * 8) = 1);
+      assert (pow2 (i * 8) * nat_from_intseq_le_ (Seq.slice b 0 len) == nat_from_intseq_le_ b) end
+    else begin
+      lemma_nat_from_bytes_le_slice len b (i - 1);
+      assert (nat_from_intseq_le_ b == nat_from_intseq_le_ (Seq.slice b 0 (i - 1)) + pow2 ((i - 1) * 8) * nat_from_intseq_le_ (Seq.slice b (i - 1) len));
+      lemma_nat_from_bytes_le_slice0 len b i;
+      assert (
+	nat_from_intseq_le_ (Seq.slice b 0 (i - 1)) + pow2 ((i - 1) * 8) * nat_from_intseq_le_ (Seq.slice b (i - 1) len) ==
+	nat_from_intseq_le_ (Seq.slice b 0 (i - 1)) + pow2 ((i - 1) * 8) * v b.[i - 1] + pow2 (i * 8) * nat_from_intseq_le_ (Seq.slice b i len));
+      let b1 = Seq.slice b 0 i in
+      lemma_nat_from_bytes_le_slice i b1 (i - 1);
+      assert (nat_from_intseq_le_ b1 == nat_from_intseq_le_ (Seq.slice b1 0 (i - 1)) + pow2 ((i - 1) * 8) * nat_from_intseq_le_ (Seq.slice b1 (i - 1) i));
+      lemma_nat_from_bytes_le_slice1 len b i
+    end
+  end
+
+val lemma_mul_pow2_and_zero: a:nat -> Lemma (pow2 a * 0 = 0)
+let lemma_mul_pow2_and_zero a = ()
+
+val nat_from_bytes_le_eq_lemma_: len:size_nat{len < 16} -> b:lseq uint8 len -> Lemma
+ (let tmp = create 16 (u8 0) in
+  BSeq.nat_from_intseq_le_ b == BSeq.nat_from_intseq_le_ (update_sub tmp 0 len b))
+let nat_from_bytes_le_eq_lemma_ len b =
+  let tmp = create 16 (u8 0) in
+  let r = update_sub tmp 0 len b in
+  assert (Seq.slice r 0 len == b);
+  assert (forall (i:nat). len <= i /\ i < 16 ==> r.[i] == u8 0);
+  assert (forall (i:nat). i < 16 - len ==> Seq.index (Seq.slice r len 16) i == u8 0);
+  lemma_nat_from_bytes_le_slice 16 r len;
+  assert (nat_from_intseq_le_ r == nat_from_intseq_le_ (Seq.slice r 0 len) + pow2 (len * 8) * nat_from_intseq_le_ (Seq.slice r len 16));
+  assert (nat_from_intseq_le_ r == nat_from_intseq_le_ b + pow2 (len * 8) * nat_from_intseq_le_ (Seq.slice r len 16));
+  lemma_nat_from_bytes_le_zeroes (16 - len) (Seq.slice r len 16);
+  assert (nat_from_intseq_le_ (Seq.slice r len 16) = 0);
+  assert (nat_from_intseq_le_ r == nat_from_intseq_le_ b + pow2 (len * 8) * 0);
+  lemma_mul_pow2_and_zero (len * 8)
+
+let nat_from_bytes_le_eq_lemma len b = nat_from_bytes_le_eq_lemma_ len b
