code/experimental/poly1305/Hacl.Impl.Poly1305.fst
@@ -113,9 +113,10 @@ val poly1305_encode_last:
 let poly1305_encode_last #s f len b =
   push_frame();
   let tmp = create 16ul (u8 0) in
-  copy (sub tmp 0ul len) (sub b 0ul len);
+  update_sub tmp 0ul len b;
   let h0 = ST.get () in
-  assume (BSeq.nat_from_bytes_le (as_seq h0 b) == BSeq.nat_from_bytes_le (as_seq h0 tmp));
+  Hacl.Impl.Poly1305.Lemmas.nat_from_bytes_le_eq_lemma (v len) (as_seq h0 b);
+  assert (BSeq.nat_from_bytes_le (as_seq h0 b) == BSeq.nat_from_bytes_le (as_seq h0 tmp));
   load_felem_le f tmp;
   let h1 = ST.get () in
   lemma_feval_is_fas_nat h1 f;
